%Identisch mit wz-2013-6-4.tex
\Aufgabe[e]{Partielle Ableitungen} {
Bestimmen Sie zu  jeder der folgenden Funktionen $\varphi:\R^n\rightarrow \R$ die ersten und zweiten Ableitungen
$$\begin{pmatrix}\frac{\partial \varphi}{\partial x_1}\\\vdots\\\frac{\partial \varphi}{\partial
x_n}\end{pmatrix},\qquad \begin{pmatrix}\frac{\partial^2 \varphi}{\partial x_1\partial
x_1}&\hdots& \frac{\partial^2\varphi}{\partial x_1 \partial x_n}\\
\vdots&\ddots&\vdots\\
\frac{\partial^2 \varphi}{\partial x_n\partial x_1}&\hdots&\frac{\partial^2 \varphi}{\partial
x_n\partial x_n}\end{pmatrix}.$$
\begin{align*}
f(x,y)=& \EH{2xy^2}&\qquad&&g(x,y)=& x^2\sin(2x+y)\\
h(x,y)=& \sin(2x)\cos(3y)&&&k(x,y,z)=&xy^2z^3\\
l(x,y)=&\frac{xy}{xy-1}
\end{align*}


}


\Loesung{
\begin{align*}
\nabla f(x,y)=& (2y^2\EH{2xy^2},\, 4xy\EH{2xy^2})^\top\\
\left( \frac{\partial^2 f}{\partial x_i\partial x_j}\right) =
& \begin{pmatrix}4y^4\EH{2xy^2}&(4y+8xy^3)\EH{2xy^2}\\
(4y+8xy^3)\EH{2xy^2}& (4x+16x^2y^2)\EH{2xy^2}\end{pmatrix}\\
\nabla g(x,y)=& (2x\sin(2x+y)+2x^2\cos(2x+y),\, x^2\cos(2x+y))^\top\\
\left( \frac{\partial^2 g}{\partial x_i\partial x_j}\right) =
& \Bigl(\begin{matrix}2\sin(2x+y)+8x\cos(2x+y)-4x^2\sin(2x+y)&\hdots\\
2x\cos(2x+y)-2x^2\sin(2x+y)&\hdots\end{matrix}\Bigr.\\
&\qquad\qquad\qquad\qquad\Bigl.\begin{matrix}\hdots& 2x\cos(2x+y)-2x^2\sin(2x+y)\\
\hdots& -x^2\sin(2x+y)\end{matrix}\Bigr)\\
\nabla h(x,y)=& (2\cos(2x)\cos(3y),\, -3\sin(2x)\sin(3y))^\top\\
\left( \frac{\partial^2 h}{\partial x_i\partial x_j}\right) =
& \begin{pmatrix}-4\sin(2x)\cos(3y)& -6\cos(2x)\sin(3y)\\
-6\cos(2x)\sin(3y)& -9\sin(2x)\cos(3y)\end{pmatrix}\\
\nabla k(x,y,z)=& (y^2z^3,\, 2xyz^3,\, 3xy^2z^2)^\top\\
\left( \frac{\partial^2 k}{\partial x_i\partial x_j}\right) =
& \begin{pmatrix}
 0       &  2yz^3  &  3y^2z^2  \\
 2yz^3   &  2xz^3  &  6xyz^2   \\
 3y^2z^2 &  6xyz^2 &  6xy^2z   \end{pmatrix}\\
\nabla l(x,y)=& \left( \frac{y(xy-1)-y\cdot xy}{(xy-1)^2},\, \frac{x(xy-1)-x\cdot
 xy}{(xy-1)^2}\right)^\top
=\left( \frac{-y}{(xy-1)^2},\, \frac{-x}{(xy-1)^2}\right)^\top\\
\left( \frac{\partial^2 l}{\partial x_i\partial x_j}\right) =
& \begin{pmatrix}
\frac{2y^2}{(xy-1)^3}& \frac{-(xy-1)^2-(-y)\cdot 2(xy-1)\cdot x}{(xy-1)^4}\\
\frac{1+xy}{(xy-1)^3}& \frac{2x^2}{(xy-1)^3}
\end{pmatrix}
=\frac 1{(xy-1)^3}\begin{pmatrix}
2y^2&1+xy\\
1+xy&2x^2
\end{pmatrix}
\end{align*}
}

\ErgebnisC{AufganalysDiffNdim001}
{
\begin{align*}
\nabla f(x,y)=& (2y^2\EH{2xy^2},\, 4xy\EH{2xy^2})^\top\\
\nabla g(x,y)=& (2x\sin(2x+y)+2x^2\cos(2x+y),\, x^2\cos(2x+y))^\top\\
\nabla h(x,y)=& (2\cos(2x)\cos(3y),\, -3\sin(2x)\sin(3y))^\top\\
\nabla k(x,y,z)=& (y^2z^3,\, 2xyz^3,\, 3xy^2z^2)^\top\\
\nabla l(x,y)=& =\left( \frac{-y}{(xy-1)^2},\, \frac{-x}{(xy-1)^2}\right)^\top
\end{align*}

}
